proof/correctness/Utils.ec
@@ -1,7 +1,79 @@
+pragma Goals : printall.
+
 require import AllCore List RealExp IntDiv.
+require import BitEncoding.
+(*---*) import BitChunking.
 
 from Jasmin require import JModel.
+
+require import RandomBytes XMSS_IMPL XMSS_IMPL_HOP1.
+
+require import Array8 Array32.
 
 pred valid_ptr (p o : W64.t) = 
   0 <= to_uint o => 
     0 <= to_uint p /\ to_uint (p + o) < W64.modulus.
+
+op BytesToBits (bytes : W8.t list) : bool list = flatten (map W8.w2bits bytes).
+op BitsToBytes (bits : bool list) : W8.t list = map W8.bits2w (chunk W8.size bits).
+
+(*** ***)                                        
+
+op addr_to_bytes (a : W32.t Array8.t) : W8.t list = 
+  let addr_bits : bool list = flatten (mkseq (fun (i : int) => W32.w2bits a.[i]) 8) in
+  BitsToBytes addr_bits.
+
+
+lemma addr_to_bytes_correctness (x : W32.t Array8.t) : 
+    hoare[M(Syscall).__addr_to_bytes : arg.`2 = x ==> to_list res = addr_to_bytes x].
+proof.
+proc.
+auto => />. 
+admit.
+qed.
+
+lemma addr_to_bytes_ll : 
+    phoare[M(Syscall).__addr_to_bytes : true ==> true] = 1%r.
+proof.
+proc; inline.
+while (true) (8 - i); auto => /> /#.
+qed.
+
+(*
+lemma addr_to_bytes_correctness (x : W32.t Array8.t) : 
+    phoare[M_Hop1(Syscall).__addr_to_bytes :
+      arg.`2 = x ==> res = Array32.of_list witness (addr_to_bytes x)] = 1%r.
+proof.
+conseq (addr_to_bytes_ll) (addr_to_bytes_correctness x).
+auto => />.
+qed.
+*)
+
+lemma addr_to_bytes_hop1 :
+    equiv [M(Syscall).__addr_to_bytes ~ M_Hop1(Syscall).__addr_to_bytes : ={arg} ==> ={res}].  
+proof. proc ; sim => />. qed.
+
+(*** Hop 1 ***)
+
+lemma addr_to_bytes_hop1_ll : phoare [ M_Hop1(Syscall).__addr_to_bytes : true ==> true] = 1%r.
+proof.
+proc ; inline.
+while (true) (8 - i); auto => /> /#.
+qed.
+
+lemma addr_to_bytes_hop1_correctness (x : W32.t Array8.t) : 
+    hoare[M_Hop1(Syscall).__addr_to_bytes : arg.`2 = x ==> to_list res = addr_to_bytes x].
+proof.
+proc.
+auto => />. 
+admit.
+qed.
+
+lemma p_addr_to_bytes_hop1_correctness (x : W32.t Array8.t) : 
+    phoare[M_Hop1(Syscall).__addr_to_bytes :
+      arg.`2 = x ==> res = Array32.of_list witness (addr_to_bytes x)] = 1%r.
+proof.
+conseq (addr_to_bytes_hop1_ll) (addr_to_bytes_hop1_correctness x); auto => /> *.
+admit.
+qed.
+
