proof/correctness/Hop2.ec
@@ -1,0 +1,134 @@
+
+pragma Goals : printall.
+
+require import AllCore List RealExp IntDiv.
+from Jasmin require import JModel JArray.
+
+require import Params Parameters Address Notation Primitives Wots Generic.
+require import RandomBytes XMSS_IMPL XMSS_IMPL_HOP1.
+
+require import Array2 Array3 Array8 Array32 Array67 Array2144.
+
+require import Utils. (* valid ptr predicate & addr_to_bytes *)
+require import Correctness_Mem. (* memcpy results *)
+(*---*) import NBytes.
+require import Termination.
+
+
+op padding_len : int.
+op prf_padding_val : W8.t.
+op prf_kg_padding_val : W8.t.
+
+module Hop2 = {
+  proc prf (in_0 : W8.t list, key : nbytes) : nbytes = {
+    var r : nbytes;
+    var padding : W8.t list;
+    var buf : W8.t list;
+
+    padding <- nseq padding_len prf_padding_val;
+    buf <- padding ++ key ++ in_0;
+
+    r <- Hash buf;
+
+    return r;
+  }
+
+  proc prf_keygen (in_0 : W8.t list, key : nbytes) : nbytes = {
+    var r : nbytes;
+    var padding : W8.t list;
+    var buf : W8.t list;
+
+    padding <- nseq padding_len prf_kg_padding_val;
+    buf <- padding ++ key ++ in_0;
+
+    r <- Hash buf;
+    
+    return r;
+
+  }
+  
+  proc thash_f (out : nbytes, seed : nbytes, address : adrs) : nbytes * adrs = {
+    var padding : W8.t list;
+    var addr_bytes : W8.t list;
+    var u : nbytes;
+    var bitmask : nbytes;
+    var buf : W8.t list;
+    var i : int;
+    var t : W8.t;
+    
+    padding <- nseq padding_len prf_padding_val;
+    addr_bytes <- addr_to_bytes address;
+    u <@ prf (addr_bytes, seed);
+
+    address <- set_key_and_mask address 1;
+    addr_bytes <- addr_to_bytes address;
+    
+    bitmask <@ prf (addr_bytes, seed);
+
+    buf <- padding ++ u ++ bitmask;
+
+    i <- 0;
+    while (i < n) {
+      t <- nth witness out i;
+      t <- (t `^` (nth witness bitmask i));
+      buf <- put buf ((32 + 32) + i) t;
+      i <- i + 1;
+    }
+
+    out <- Hash buf;
+
+    return (out, address);
+  } 
+
+  proc chain(X : nbytes, i s : int, _seed : seed, address : adrs) : nbytes * adrs = {
+    var t : nbytes <- X;
+    var chain_count : int <- 0;
+    var _key : key;
+    var bitmask : nbytes;
+    var addr_bytes : W8.t list;
+
+    while (chain_count < s) {
+      address <- set_hash_addr address (i + chain_count);
+      address <- set_key_and_mask address 0;
+
+      _key <- PRF _seed address;
+      address <- set_key_and_mask address 1;
+      
+      addr_bytes <- addr_to_bytes address;
+      
+      bitmask <@ prf(_seed, addr_bytes);
+      
+      (t, address) <@ thash_f (t, _seed, address);
+      
+      chain_count <- chain_count + 1;
+    }
+    
+    return (t, address);
+   }
+}.
+
+
+lemma prf_hop2 (a b : W8.t Array32.t) :
+    equiv [
+    M(Syscall).__prf ~ Hop2.prf : 
+    arg{1}.`2 = a /\ arg{1}.`2 = b /\ arg{2} = (to_list a, to_list b) 
+    ==>
+    res{2} = to_list res{1}
+    ].
+proof.
+proc.
+admit.
+qed.
+
+
+lemma prf_hop2 (a b : W8.t Array32.t) :
+    equiv [
+    M(Syscall).__prf ~ Hop2.prf : 
+    arg{1}.`2 = a /\ arg{1}.`2 = b /\ arg{2} = (to_list a, to_list b) 
+    ==>
+    res{2} = to_list res{1}
+    ].
+proof.
+proc.
+admit.
+qed.
