proof/extraction/XMSS_IMPL.ec
@@ -1104,19 +1104,6 @@ module M(SC:Syscall_t) = {
     return (a);
   }
   
-  proc __memset_u8_128 (a:W8.t Array128.t, value:W8.t) : W8.t Array128.t = {
-    
-    var i:W64.t;
-    
-    i <- (W64.of_int 0);
-    
-    while ((i \ult (W64.of_int 128))) {
-      a.[(W64.to_uint i)] <- value;
-      i <- (i + (W64.of_int 1));
-    }
-    return (a);
-  }
-  
   proc __memset_u8_4 (a:W8.t Array4.t, value:W8.t) : W8.t Array4.t = {
     
     var i:W64.t;
@@ -1124,6 +1111,19 @@ module M(SC:Syscall_t) = {
     i <- (W64.of_int 0);
     
     while ((i \ult (W64.of_int 4))) {
+      a.[(W64.to_uint i)] <- value;
+      i <- (i + (W64.of_int 1));
+    }
+    return (a);
+  }
+  
+  proc __memset_u8_128 (a:W8.t Array128.t, value:W8.t) : W8.t Array128.t = {
+    
+    var i:W64.t;
+    
+    i <- (W64.of_int 0);
+    
+    while ((i \ult (W64.of_int 128))) {
       a.[(W64.to_uint i)] <- value;
       i <- (i + (W64.of_int 1));
     }
@@ -1158,6 +1158,20 @@ module M(SC:Syscall_t) = {
     return (out);
   }
   
+  proc __memcpy_u8u8_64_32 (out:W8.t Array64.t, in_0:W8.t Array32.t) : 
+  W8.t Array64.t = {
+    
+    var i:W64.t;
+    
+    i <- (W64.of_int 0);
+    
+    while ((i \ult (W64.of_int 32))) {
+      out.[(W64.to_uint i)] <- in_0.[(W64.to_uint i)];
+      i <- (i + (W64.of_int 1));
+    }
+    return (out);
+  }
+  
   proc __memcpy_u8u8_64_64 (out:W8.t Array64.t, in_0:W8.t Array64.t) : 
   W8.t Array64.t = {
     
@@ -1186,17 +1200,12 @@ module M(SC:Syscall_t) = {
     return (out);
   }
   
-  proc __memcpy_u8u8_64_32 (out:W8.t Array64.t, in_0:W8.t Array32.t) : 
+  proc _memcpy_u8u8_64_32 (out:W8.t Array64.t, in_0:W8.t Array32.t) : 
   W8.t Array64.t = {
     
-    var i:W64.t;
     
-    i <- (W64.of_int 0);
     
-    while ((i \ult (W64.of_int 32))) {
-      out.[(W64.to_uint i)] <- in_0.[(W64.to_uint i)];
-      i <- (i + (W64.of_int 1));
-    }
+    out <@ __memcpy_u8u8_64_32 (out, in_0);
     return (out);
   }
   
@@ -1218,12 +1227,15 @@ module M(SC:Syscall_t) = {
     return (out);
   }
   
-  proc _memcpy_u8u8_64_32 (out:W8.t Array64.t, in_0:W8.t Array32.t) : 
+  proc _x_memcpy_u8u8_64_32 (out:W8.t Array64.t, in_0:W8.t Array32.t) : 
   W8.t Array64.t = {
     
     
     
-    out <@ __memcpy_u8u8_64_32 (out, in_0);
+    out <- out;
+    in_0 <- in_0;
+    out <@ _memcpy_u8u8_64_32 (out, in_0);
+    out <- out;
     return (out);
   }
   
@@ -1247,18 +1259,6 @@ module M(SC:Syscall_t) = {
     out <- out;
     in_0 <- in_0;
     out <@ _memcpy_u8u8_32_32 (out, in_0);
-    out <- out;
-    return (out);
-  }
-  
-  proc _x_memcpy_u8u8_64_32 (out:W8.t Array64.t, in_0:W8.t Array32.t) : 
-  W8.t Array64.t = {
-    
-    
-    
-    out <- out;
-    in_0 <- in_0;
-    out <@ _memcpy_u8u8_64_32 (out, in_0);
     out <- out;
     return (out);
   }
@@ -1295,8 +1295,8 @@ module M(SC:Syscall_t) = {
     return (out);
   }
   
-  proc __memcpy_u8u8_2_64_2144 (out:W8.t Array64.t, in_0:W8.t Array2144.t,
-                                in_offset:W64.t, bytes:W64.t) : W8.t Array64.t *
+  proc __memcpy_u8u8_2_32_2144 (out:W8.t Array32.t, in_0:W8.t Array2144.t,
+                                in_offset:W64.t, bytes:W64.t) : W8.t Array32.t *
                                                                 W64.t = {
     
     var i:W64.t;
@@ -1311,8 +1311,8 @@ module M(SC:Syscall_t) = {
     return (out, in_offset);
   }
   
-  proc __memcpy_u8u8_2_32_2144 (out:W8.t Array32.t, in_0:W8.t Array2144.t,
-                                in_offset:W64.t, bytes:W64.t) : W8.t Array32.t *
+  proc __memcpy_u8u8_2_64_2144 (out:W8.t Array64.t, in_0:W8.t Array2144.t,
+                                in_offset:W64.t, bytes:W64.t) : W8.t Array64.t *
                                                                 W64.t = {
     
     var i:W64.t;
@@ -1593,14 +1593,12 @@ module M(SC:Syscall_t) = {
     
     var buf:W8.t Array96.t;
     var padding_buf:W8.t Array32.t;
-    var offset:W64.t;
     buf <- witness;
     padding_buf <- witness;
     padding_buf <- (Array32.init (fun i => buf.[0 + i]));
     padding_buf <@ __ull_to_bytes_32 (padding_buf, (W64.of_int 3));
     buf <- Array96.init
            (fun i => if 0 <= i < 0 + 32 then padding_buf.[i-0] else buf.[i]);
-    offset <- (W64.of_int 32);
     aux <@ _x_memcpy_u8u8_32_32 ((Array32.init (fun i => buf.[32 + i])),
     key);
     buf <- Array96.init
@@ -1610,7 +1608,7 @@ module M(SC:Syscall_t) = {
     buf <- Array96.init
            (fun i => if (32 + 32) <= i < (32 + 32) + 32
            then aux.[i-(32 + 32)] else buf.[i]);
-    out <@ __core_hash_96 (out, buf);
+    out <@ __core_hash__96 (out, buf);
     return (out);
   }
   
@@ -2013,8 +2011,7 @@ module M(SC:Syscall_t) = {
     return (out, addr);
   }
   
-  proc __base_w_67_32 (output:W32.t Array67.t, input:W8.t Array32.t) : 
-  W32.t Array67.t = {
+  proc __base_w_3_2 (output:W32.t Array3.t, input:W8.t Array2.t) : W32.t Array3.t = {
     var aux: int;
     
     var in_0:W64.t;
@@ -2029,7 +2026,7 @@ module M(SC:Syscall_t) = {
     bits <- (W64.of_int 0);
     total <- (W8.of_int 0);
     consumed <- 0;
-    while (consumed < 67) {
+    while (consumed < 3) {
       if ((bits = (W64.of_int 0))) {
         total <- input.[(W64.to_uint in_0)];
         in_0 <- (in_0 + (W64.of_int 1));
@@ -2048,7 +2045,8 @@ module M(SC:Syscall_t) = {
     return (output);
   }
   
-  proc __base_w_3_2 (output:W32.t Array3.t, input:W8.t Array2.t) : W32.t Array3.t = {
+  proc __base_w_67_32 (output:W32.t Array67.t, input:W8.t Array32.t) : 
+  W32.t Array67.t = {
     var aux: int;
     
     var in_0:W64.t;
@@ -2063,7 +2061,7 @@ module M(SC:Syscall_t) = {
     bits <- (W64.of_int 0);
     total <- (W8.of_int 0);
     consumed <- 0;
-    while (consumed < 3) {
+    while (consumed < 67) {
       if ((bits = (W64.of_int 0))) {
         total <- input.[(W64.to_uint in_0)];
         in_0 <- (in_0 + (W64.of_int 1));
